FOmegaC/SpecTyping.v
@@ -7,19 +7,19 @@ Reserved Notation "⟨ x : τ ∈ Γ ⟩"
     τ at level 98,
     Γ at level 98).
 
-Inductive GetEVar : Env → Ix → Tm → Prop :=
-  | ge_here {Γ τ} :
+Inductive GetTmVar : Env → Ix → Exp → Prop :=
+  | tm_here {Γ τ} :
       ⟨   O : τ[wkm] ∈ Γ ▻ τ ⟩
-  | ge_there_evar {Γ x τ τ'} :
+  | tm_there_evar {Γ x τ τ'} :
       ⟨   x : τ      ∈ Γ      ⟩ →
       ⟨ S x : τ[wkm] ∈ Γ ▻ τ' ⟩
-  | ge_there_τvar {Γ x τ k'} :
+  | tm_there_τvar {Γ x τ k'} :
       ⟨   x : τ      ∈ Γ      ⟩ →
       ⟨ S x : τ[wkm] ∈ Γ ► k' ⟩
-  | ge_there_γvar {Γ x τ τ1' τ2' k'} :
+  | tm_there_γvar {Γ x τ τ1' τ2' k'} :
       ⟨   x : τ      ∈ Γ      ⟩ →
       ⟨ S x : τ[wkm] ∈ Γ ◅ τ1' ~ τ2' ∷ k' ⟩
-where "⟨ x : τ ∈ Γ ⟩" := (GetEVar Γ x τ).
+where "⟨ x : τ ∈ Γ ⟩" := (GetTmVar Γ x τ).
 
 Reserved Notation "⟨ α ∷ k ∈ Γ ⟩"
   ( at level 0,
@@ -27,19 +27,19 @@ Reserved Notation "⟨ α ∷ k ∈ Γ ⟩"
     k at level 98,
     Γ at level 98).
 
-Inductive GetTVar : Env → Ix → Kind → Prop :=
-  | gt_here {Γ k} :
+Inductive GetTyVar : Env → Ix → Kind → Prop :=
+  | ty_here {Γ k} :
       ⟨   O ∷ k ∈ Γ ► k ⟩
-  | gt_there_evar {Γ α k τ'} :
+  | ty_there_evar {Γ α k τ'} :
       ⟨   α ∷ k ∈ Γ      ⟩ →
       ⟨ S α ∷ k ∈ Γ ▻ τ' ⟩
-  | gt_there_τvar {Γ α k k'} :
+  | ty_there_τvar {Γ α k k'} :
       ⟨   α ∷ k ∈ Γ      ⟩ →
       ⟨ S α ∷ k ∈ Γ ► k' ⟩
-  | gt_there_γvar {Γ α k τ1' τ2' k'} :
+  | ty_there_γvar {Γ α k τ1' τ2' k'} :
       ⟨   α ∷ k ∈ Γ      ⟩ →
       ⟨ S α ∷ k ∈ Γ ◅ τ1' ~ τ2' ∷ k' ⟩
-where "⟨ α ∷ k ∈ Γ ⟩" := (GetTVar Γ α k).
+where "⟨ α ∷ k ∈ Γ ⟩" := (GetTyVar Γ α k).
 
 Reserved Notation "⟨ c : τ1 ~ τ2 ∷ k ∈ Γ ⟩"
   ( at level 0,
@@ -49,19 +49,19 @@ Reserved Notation "⟨ c : τ1 ~ τ2 ∷ k ∈ Γ ⟩"
     k at level 98,
     Γ at level 98).
 
-Inductive GetCVar : Env → Ix → Tm → Tm → Kind → Prop :=
-  | gc_here {Γ τ1 τ2 k} :
+Inductive GetCoVar : Env → Ix → Exp → Exp → Kind → Prop :=
+  | co_here {Γ τ1 τ2 k} :
       ⟨   O : τ1[wkm] ~ τ2[wkm] ∷ k ∈ Γ ◅ τ1 ~ τ2 ∷ k ⟩
-  | gc_there_evar {Γ c τ1 τ2 k τ'} :
+  | co_there_evar {Γ c τ1 τ2 k τ'} :
       ⟨   c : τ1      ~ τ2      ∷ k ∈ Γ      ⟩ →
       ⟨ S c : τ1[wkm] ~ τ2[wkm] ∷ k ∈ Γ ▻ τ' ⟩
-  | gc_there_τvar {Γ c τ1 τ2 k k'} :
+  | co_there_τvar {Γ c τ1 τ2 k k'} :
       ⟨   c : τ1      ~ τ2      ∷ k ∈ Γ      ⟩ →
       ⟨ S c : τ1[wkm] ~ τ2[wkm] ∷ k ∈ Γ ► k' ⟩
-  | gc_there_γvar {Γ c τ1 τ2 k τ1' τ2' k'} :
+  | co_there_γvar {Γ c τ1 τ2 k τ1' τ2' k'} :
       ⟨   c : τ1      ~ τ2      ∷ k ∈ Γ      ⟩ →
       ⟨ S c : τ1[wkm] ~ τ2[wkm] ∷ k ∈ Γ ◅ τ1' ~ τ2' ∷ k' ⟩
-where "⟨ c : τ1 ~ τ2 ∷ k ∈ Γ ⟩" := (GetCVar Γ c τ1 τ2 k).
+where "⟨ c : τ1 ~ τ2 ∷ k ∈ Γ ⟩" := (GetCoVar Γ c τ1 τ2 k).
 
 Reserved Notation "⟨ Γ ⊢ τ ∷ k ⟩"
   ( at level 0,
@@ -69,28 +69,28 @@ Reserved Notation "⟨ Γ ⊢ τ ∷ k ⟩"
     τ at level 98,
     k at level 98).
 
-Inductive OfKind (Γ: Env) : Tm → Kind → Prop :=
-  | K_tvar {α k} :
+Inductive Ty (Γ: Env) : Exp → Kind → Prop :=
+  | TyVar {α k} :
       ⟨ α ∷ k ∈ Γ ⟩ →
       ⟨ Γ ⊢ var α ∷ k ⟩
-  | K_absττ {τ k1 k2} :
+  | TAbs {τ k1 k2} :
       ⟨ Γ ► k1 ⊢ τ ∷ k2 ⟩ →
-      ⟨ Γ ⊢ absττ k1 τ ∷ karr k1 k2 ⟩
-  | K_appττ {τ1 τ2 k1 k2}:
+      ⟨ Γ ⊢ τabs k1 τ ∷ karr k1 k2 ⟩
+  | TApp {τ1 τ2 k1 k2}:
       ⟨ Γ ⊢ τ1 ∷ karr k1 k2 ⟩ →
       ⟨ Γ ⊢ τ2 ∷ k1 ⟩ →
-      ⟨ Γ ⊢ appττ τ1 τ2 ∷ k2 ⟩
-  | K_arree {τ1 τ2} :
+      ⟨ Γ ⊢ τapp τ1 τ2 ∷ k2 ⟩
+  | Arr {τ1 τ2} :
       ⟨ Γ ⊢ τ1 ∷ kstar ⟩  →
       ⟨ Γ ⊢ τ2 ∷ kstar ⟩  →
-      ⟨ Γ ⊢ arree τ1 τ2 ∷ kstar ⟩
-  | K_arrτe {τ k} :
+      ⟨ Γ ⊢ arr τ1 τ2 ∷ kstar ⟩
+  | Arrτ {τ k} :
       ⟨ Γ ► k ⊢ τ ∷ kstar ⟩  →
-      ⟨ Γ ⊢ arrτe k τ ∷ kstar ⟩
-  | K_arrγe {τ1 τ2 τ3 k} :
-      ⟨ Γ ◅ τ1 ~ τ2 ∷ k ⊢ τ3 ∷ kstar ⟩  →
-      ⟨ Γ ⊢ arrγe τ1 τ2 k τ3 ∷ kstar ⟩
-where "⟨ Γ ⊢ τ ∷ k ⟩" := (OfKind Γ τ k).
+      ⟨ Γ ⊢ arrτ k τ ∷ kstar ⟩
+  | Arrγ {τ1 τ2 τ3 k} :
+      ⟨ Γ ⊢ τ3 ∷ kstar ⟩  →
+      ⟨ Γ ⊢ arrγ τ1 τ2 k τ3 ∷ kstar ⟩
+where "⟨ Γ ⊢ τ ∷ k ⟩" := (Ty Γ τ k).
 
 Reserved Notation "⟨ Γ ⊢ γ : τ1 ~ τ2 ∷ k ⟩"
   ( at level 0,
@@ -100,74 +100,77 @@ Reserved Notation "⟨ Γ ⊢ γ : τ1 ~ τ2 ∷ k ⟩"
     τ2 at level 98,
     k at level 98).
 
-Inductive OfProp (Γ: Env) : Tm → Tm → Tm → Kind → Prop :=
-  | R_τvar {α k} :
+Inductive Co (Γ: Env) : Exp → Exp → Exp → Kind → Prop :=
+  | CoTyVar {α k} :
       ⟨ α ∷ k ∈ Γ ⟩ →
       ⟨ Γ ⊢ var α : var α ~ var α ∷ k ⟩
-  | R_cvar {c τ1 τ2 k} :
+  | CoVar {c τ1 τ2 k} :
       ⟨ c : τ1 ~ τ2 ∷ k ∈ Γ ⟩ →
       ⟨ Γ ⊢ var c : τ1 ~ τ2 ∷ k ⟩
-  | R_γabsττ {γ τ1 τ2 k1 k2} :
+  | CoTAbs {γ τ1 τ2 k1 k2} :
       ⟨ Γ ► k1 ⊢ γ : τ1 ~ τ2 ∷ k2 ⟩ →
-      ⟨ Γ ⊢ γabsττ k1 γ : absττ k1 τ1 ~ absττ k1 τ2 ∷ karr k1 k2 ⟩
-  | R_γappττ {γ1 γ2 τ11 τ12 τ21 τ22 k1 k2 }:
+      ⟨ Γ ⊢ coτabs k1 γ : τabs k1 τ1 ~ τabs k1 τ2 ∷ karr k1 k2 ⟩
+  | CoTApp {γ1 γ2 τ11 τ12 τ21 τ22 k1 k2 }:
       ⟨ Γ ⊢ γ1 : τ11 ~ τ21 ∷ karr k1 k2 ⟩ →
       ⟨ Γ ⊢ γ2 : τ12 ~ τ22 ∷ k1 ⟩ →
-      ⟨ Γ ⊢ γappττ γ1 γ2 : appττ τ11 τ12 ~ appττ τ21 τ22 ∷ k2 ⟩
-  | R_γarree {γ1 γ2 τ11 τ12 τ21 τ22}:
+      ⟨ Γ ⊢ coτapp γ1 γ2 : τapp τ11 τ12 ~ τapp τ21 τ22 ∷ k2 ⟩
+  | CoArr {γ1 γ2 τ11 τ12 τ21 τ22}:
       ⟨ Γ ⊢ γ1 : τ11 ~ τ21 ∷ kstar ⟩ →
       ⟨ Γ ⊢ γ2 : τ12 ~ τ22 ∷ kstar ⟩ →
-      ⟨ Γ ⊢ γarree γ1 γ2 : arree τ11 τ21 ~ arree τ21 τ22 ∷ kstar ⟩
-  | R_γarrτe {γ τ1 τ2 k} :
+      ⟨ Γ ⊢ coarr γ1 γ2 : arr τ11 τ21 ~ arr τ21 τ22 ∷ kstar ⟩
+  | CoArrτ {γ τ1 τ2 k} :
       ⟨ Γ ► k ⊢ γ : τ1 ~ τ2 ∷ kstar ⟩ →
-      ⟨ Γ ⊢ γarrτe k γ : arrτe k τ1 ~ arrτe k τ2 ∷ kstar ⟩
-  | R_γbeta {γ1 γ2 τ11 τ12 τ21 τ22 k1 k2} :
+      ⟨ Γ ⊢ coarrτ k γ : arrτ k τ1 ~ arrτ k τ2 ∷ kstar ⟩
+  | CoArrγ {γ τ1 τ2 τ3 τ4 k} :
+      ⟨ Γ ⊢ γ : τ3 ~ τ4 ∷ kstar ⟩ →
+      ⟨ Γ ⊢ coarrγ τ1 τ2 k γ : arrγ τ1 τ2 k τ3 ~ arrγ τ1 τ2 k τ4 ∷ kstar ⟩
+  | CoBeta {γ1 γ2 τ11 τ12 τ21 τ22 k1 k2} :
       ⟨ Γ ► k1 ⊢ γ1 : τ11 ~ τ21 ∷ k2 ⟩ →
       ⟨ Γ ⊢ γ2 : τ12 ~ τ22 ∷ k1 ⟩ →
-      ⟨ Γ ⊢ γbeta γ1 γ2 : appττ (absττ k1 τ11) τ12 ~ τ21[beta1 τ22] ∷ k2 ⟩
-  | R_γsym {γ τ1 τ2 k} :
+      ⟨ Γ ⊢ cobeta γ1 γ2 : τapp (τabs k1 τ11) τ12 ~ τ21[beta1 τ22] ∷ k2 ⟩
+  | CoSym {γ τ1 τ2 k} :
       ⟨ Γ ⊢ γ : τ1 ~ τ2 ∷ k ⟩ →
-      ⟨ Γ ⊢ γsym γ : τ2 ~ τ1 ∷ k ⟩
-  | R_γtrans {γ1 γ2 τ1 τ2 τ3 k} :
+      ⟨ Γ ⊢ cosym γ : τ2 ~ τ1 ∷ k ⟩
+  | CoTrans {γ1 γ2 τ1 τ2 τ3 k} :
       ⟨ Γ ⊢ γ1 : τ1 ~ τ2 ∷ k ⟩ →
       ⟨ Γ ⊢ γ2 : τ2 ~ τ3 ∷ k ⟩ →
-      ⟨ Γ ⊢ γtrans γ1 γ2 : τ1 ~ τ3 ∷ k ⟩
-where "⟨ Γ ⊢ γ : τ1 ~ τ2 ∷ k ⟩" := (OfProp Γ γ τ1 τ2 k).
+      ⟨ Γ ⊢ cotrans γ1 γ2 : τ1 ~ τ3 ∷ k ⟩
+where "⟨ Γ ⊢ γ : τ1 ~ τ2 ∷ k ⟩" := (Co Γ γ τ1 τ2 k).
 
-Reserved Notation "⟨ Γ ⊢ e : τ ⟩"
+Reserved Notation "⟨ Γ ⊢ s : τ ⟩"
   ( at level 0,
     Γ at level 98,
-    e at level 98,
+    s at level 98,
     τ at level 98).
 
-Inductive OfType (Γ: Env) : Tm → Tm → Prop :=
-  | T_evar {x τ} :
+Inductive Tm (Γ: Env) : Exp → Exp → Prop :=
+  | Var {x τ} :
       ⟨ x : τ ∈ Γ ⟩ →
       ⟨ Γ ⊢ var x : τ ⟩
-  | T_absee {e τ1 τ2} :
+  | Abse {s τ1 τ2} :
       ⟨ Γ ⊢ τ1 ∷ kstar ⟩ →
-      ⟨ Γ ▻ τ1 ⊢ e : τ2 ⟩ →
-      ⟨ Γ ⊢ absee τ1 e : arree τ1 τ2 ⟩
-  | T_absτe {e τ k} :
-      ⟨ Γ ► k ⊢ e : τ ⟩ →
-      ⟨ Γ ⊢ absτe k e : arrτe k τ ⟩
-  | T_absγe {e τ1 τ2 τ3 k} :
-      ⟨ Γ ◅ τ1 ~ τ2 ∷ k ⊢ e : τ3 ⟩ →
-      ⟨ Γ ⊢ absγe τ1 τ2 k e : arrγe τ1 τ2 k τ3 ⟩
-  | T_appee {e1 e2 τ1 τ2} :
-      ⟨ Γ ⊢ e1 : arree τ1 τ2 ⟩ →
-      ⟨ Γ ⊢ e2 : τ1 ⟩ →
-      ⟨ Γ ⊢ appee e1 e2 : τ2 ⟩
-  | T_appeτ {e τ1 τ2 k} :
-      ⟨ Γ ⊢ e : arrτe k τ1 ⟩ →
+      ⟨ Γ ▻ τ1 ⊢ s : τ2[wkm] ⟩ →
+      ⟨ Γ ⊢ abs τ1 s : arr τ1 τ2 ⟩
+  | Absτ {s τ k} :
+      ⟨ Γ ► k ⊢ s : τ ⟩ →
+      ⟨ Γ ⊢ absτ k s : arrτ k τ ⟩
+  | Absγ {s τ1 τ2 τ3 k} :
+      ⟨ Γ ◅ τ1 ~ τ2 ∷ k ⊢ s : τ3[wkm] ⟩ →
+      ⟨ Γ ⊢ absγ τ1 τ2 k s : arrγ τ1 τ2 k τ3 ⟩
+  | App {s1 s2 τ1 τ2} :
+      ⟨ Γ ⊢ s1 : arr τ1 τ2 ⟩ →
+      ⟨ Γ ⊢ s2 : τ1 ⟩ →
+      ⟨ Γ ⊢ app s1 s2 : τ2 ⟩
+  | Appτ {s τ1 τ2 k} :
+      ⟨ Γ ⊢ s : arrτ k τ1 ⟩ →
       ⟨ Γ ⊢ τ2 ∷ k ⟩ →
-      ⟨ Γ ⊢ appeτ e τ2 : τ1[beta1 τ2] ⟩
-  | T_appeγ {e γ τ1 τ2 τ3 k} :
-      ⟨ Γ ⊢ e : arrγe τ1 τ2 k τ3 ⟩ →
+      ⟨ Γ ⊢ appτ s τ2 : τ1[beta1 τ2] ⟩
+  | Appγ {s γ τ1 τ2 τ3 k} :
+      ⟨ Γ ⊢ s : arrγ τ1 τ2 k τ3 ⟩ →
       ⟨ Γ ⊢ γ : τ1 ~ τ2 ∷ k ⟩ →
-      ⟨ Γ ⊢ appeτ e γ : τ3 ⟩
-  | T_cast {e γ τ1 τ2} :
-      ⟨ Γ ⊢ e : τ1 ⟩ →
+      ⟨ Γ ⊢ appγ s γ : τ3 ⟩
+  | Cast {s γ τ1 τ2} :
+      ⟨ Γ ⊢ s : τ1 ⟩ →
       ⟨ Γ ⊢ γ : τ1 ~ τ2 ∷ kstar ⟩ →
-      ⟨ Γ ⊢ cast e γ : τ2 ⟩
-where "⟨ Γ ⊢ e : τ ⟩" := (OfType Γ e τ).
+      ⟨ Γ ⊢ cast s γ : τ2 ⟩
+where "⟨ Γ ⊢ s : τ ⟩" := (Tm Γ s τ).
